LoL/MProp/Instances.lean
@@ -5,12 +5,23 @@ instance : Nonempty PProp := ⟨PProp.mk True⟩
 
 instance : MPropPartialOrder Id Prop where
   μ := (·.prop)
-  μ_surjective := by exists (fun x => PProp.mk x); simp [Function.LeftInverse]
+  ι := fun x => PProp.mk x
+  μ_surjective := by simp [Function.LeftInverse]
+  μ_pure_injective := by simp
   μ_top := by simp
   μ_bot := by simp
   μ_nontriv := by simp
   μ_ord_pure := by simp
   μ_ord_bind := by solve_by_elim
+
+instance : MPropDetertministic Id Prop where
+  demonic := by
+    intros α c p q;
+    simp [MProp.lift, MProp.ι, MProp.μ_surjective, MProp.μ, MPropPartialOrder.ι, MPropPartialOrder.μ]
+  angelic := by
+    intros α c p q;
+    simp [MProp.lift, MProp.ι, MProp.μ_surjective, MProp.μ, MPropPartialOrder.ι, MPropPartialOrder.μ]
+
 
 instance (σ : Type) (l : Type) (m : Type -> Type)
   [Inhabited σ]
@@ -19,10 +30,10 @@ instance (σ : Type) (l : Type) (m : Type -> Type)
   μ := fun sp s => Prod.fst <$> sp s |> inst.μ
   μ_top := by intros x s; simp [pure, StateT.pure]; apply inst.μ_top
   μ_bot := by intros x s; simp [pure, StateT.pure]; apply inst.μ_bot
-  μ_surjective := by
-    exists fun sp s => (·, s) <$> MProp.ι (sp s)
-    intro x; simp [funext_iff];
-    intro s; apply inst.μ_surjective.property
+  ι := fun sp s => (·, s) <$> MProp.ι (sp s)
+  μ_surjective := by intro x; simp [funext_iff]; intro s; apply inst.μ_surjective
+  μ_pure_injective := by
+    simp [pure, StateT.pure, MProp.ι, inst.μ_pure_injective]; intro p; rfl
   μ_ord_pure := by
     intros p₁ p₂ imp s; simp [pure, StateT.pure]
     solve_by_elim [MPropPartialOrder.μ_ord_pure]
@@ -36,15 +47,38 @@ instance (σ : Type) (l : Type) (m : Type -> Type)
     simp only [Function.comp, Pi.hasLe, <-map_bind] at leM
     apply leM; simp only [implies_true, le]
 
+instance (σ : Type) (l : Type) (m : Type -> Type)
+  [Inhabited σ]
+  [Lattice l]
+  [Monad m] [LawfulMonad m] [inst: MPropPartialOrder m l] [inst': MPropDetertministic m l]
+   : MPropDetertministic (StateT σ m) (σ -> l) where
+    demonic := by
+      intros α c p q s;
+      simp [MProp.lift, MProp.μ, MPropPartialOrder.μ]
+      simp [bind, StateT.bind]; simp [MProp.ι, MPropPartialOrder.ι]
+      have h := inst'.demonic (α := α × σ) (c := c s) (p := fun x => p x.1 x.2) (q := fun x => q x.1 x.2)
+      simp [MProp.lift, MProp.ι, MProp.μ] at h
+      apply h
+    angelic := by
+      intros α c p q s;
+      simp [MProp.lift, MProp.μ, MPropPartialOrder.μ]
+      simp [bind, StateT.bind]; simp [MProp.ι, MPropPartialOrder.ι]
+      have h := inst'.angelic (α := α × σ) (c := c s) (p := fun x => p x.1 x.2) (q := fun x => q x.1 x.2)
+      simp [MProp.lift, MProp.ι, MProp.μ] at h
+      apply h
+
 instance (ρ : Type) (l : Type) (m : Type -> Type)
   [Inhabited ρ]
   [PartialOrder l]
   [Monad m] [LawfulMonad m] [inst: MPropPartialOrder m l] : MPropPartialOrder (ReaderT ρ m) (ρ -> l) where
   μ := fun rp r => rp r |> inst.μ
+  ι := fun rp r => MProp.ι (rp r)
   μ_surjective := by
-    exists fun rp r => MProp.ι (rp r)
     intro x; simp [funext_iff];
-    intro r; apply inst.μ_surjective.property
+    intro r; apply inst.μ_surjective
+  μ_pure_injective := by
+    simp [MProp.ι, pure, ReaderT.pure, inst.μ_pure_injective]
+    intro p; rfl
   μ_top := by intros x s; simp [pure]; apply inst.μ_top
   μ_bot := by intros x s; simp [pure]; apply inst.μ_bot
   μ_ord_pure := by
@@ -60,6 +94,27 @@ instance (ρ : Type) (l : Type) (m : Type -> Type)
     simp only [Function.comp, Pi.hasLe, <-map_bind] at leM
     apply leM; simp only [implies_true, le]
 
+instance (σ : Type) (l : Type) (m : Type -> Type)
+  [Inhabited σ]
+  [Lattice l]
+  [Monad m] [LawfulMonad m] [inst: MPropPartialOrder m l] [inst': MPropDetertministic m l]
+   : MPropDetertministic (ReaderT σ m) (σ -> l) where
+  demonic := by
+      intros α c p q s;
+      simp [MProp.lift, MProp.μ, MPropPartialOrder.μ]
+      simp [bind, ReaderT.bind]
+      simp [MProp.ι, MProp.μ_surjective, MPropPartialOrder.μ_surjective]
+      have h := inst'.demonic (α := α) (c := c s) (p := fun x => p x s) (q := fun x => q x s)
+      simp [MProp.lift, MProp.ι, MProp.μ, MProp.μ_surjective] at h
+      apply h
+  angelic := by
+      intros α c p q s;
+      simp [MProp.lift, MProp.μ, MPropPartialOrder.μ]
+      simp [bind, ReaderT.bind]
+      simp [MProp.ι, MProp.μ_surjective, MPropPartialOrder.μ_surjective]
+      have h := inst'.angelic (α := α) (c := c s) (p := fun x => p x s) (q := fun x => q x s)
+      simp [MProp.lift, MProp.ι, MProp.μ, MProp.μ_surjective] at h
+      apply h
 
 abbrev Except.getD {ε α} (default : α)  : Except ε α -> α
   | Except.ok p => p
@@ -78,9 +133,11 @@ def MPropExcept (df : Prop) (ε : Type) (l : Type) (m : Type -> Type)
   μ := fun e => inst.μ $ Except.getD df <$> e
   μ_top := by intros x; simp [pure, ExceptT.pure, ExceptT.mk]; apply inst.μ_top
   μ_bot := by intros x; simp [pure, ExceptT.pure, ExceptT.mk]; apply inst.μ_bot
+  ι := fun x => Functor.map (β := Except _ _) .ok (MProp.ι x)
   μ_surjective := by
-    exists fun x => Functor.map (β := Except _ _) .ok (MProp.ι x)
-    intro x; simp [funext_iff]; apply inst.μ_surjective.property
+    intro x; simp [funext_iff]; apply inst.μ_surjective
+  μ_pure_injective := by
+    simp [pure, ExceptT.pure, ExceptT.mk, MProp.ι, inst.μ_pure_injective]
   μ_nontriv := by
     simp [pure, ExceptT.pure, Except.getD, ExceptT.mk, funext_iff];
     solve_by_elim [MPropPartialOrder.μ_nontriv]
@@ -102,6 +159,77 @@ scoped
 instance (ε : Type) (l : Type) (m : Type -> Type)
   [PartialOrder l]
   [Monad m] [LawfulMonad m] [inst: MPropPartialOrder m l] : MPropPartialOrder (ExceptT ε m) l := MPropExcept True ε l m
+
+def MPropExceptDetertministic (ε : Type) (l : Type) (m : Type -> Type)
+  [Lattice l]
+  [Monad m] [LawfulMonad m] [inst: MPropPartialOrder m l]
+  [inst': MPropDetertministic m l] : MPropDetertministic (ExceptT ε m) l where
+  demonic := by
+    intros α c p q
+    simp [MProp.lift, MProp.μ, MPropPartialOrder.μ]
+    simp [bind, ExceptT.bind, ExceptT.mk]; unfold ExceptT.bindCont
+    simp [MProp.ι, MPropPartialOrder.ι]
+    simp [instMPropPartialOrderExceptTOfLawfulMonad, MPropExcept, MProp.ι]
+    have h := inst'.demonic (α := Except ε α) (c := c)
+      (p := fun e =>
+        match e with
+        | Except.ok a    => p a
+        | Except.error e => ⌜True⌝ )
+      (q := fun e =>
+        match e with
+        | Except.ok a    => q a
+        | Except.error e => ⌜True⌝ )
+    simp [MProp.lift, MProp.ι, MProp.μ, MProp.μ_surjective] at h
+    have h₁ : ∀ p : α -> l,
+      (do
+        bind (m := m) c fun a =>
+        Except.getD { prop := True } <$>
+            match a with
+            | Except.ok a => Except.ok <$> MPropPartialOrder.ι (p a)
+            | Except.error e => pure (Except.error e)) =
+      (do
+        bind (m := m) c fun a =>
+        (MPropPartialOrder.ι $ match a with
+            | Except.ok a =>  (p a)
+            | Except.error e => ⌜True⌝)) := by
+      intro p; congr; ext a; cases a <;> simp
+      simp [Except.getD, MProp.pure, MProp.μ, inst.μ_pure_injective]
+    (repeat erw [h₁]); clear h₁; apply le_trans; apply h
+    apply le_of_eq; congr; ext a; cases a <;> simp
+  angelic := by
+    intros α c p q
+    simp [MProp.lift, MProp.μ, MPropPartialOrder.μ]
+    simp [bind, ExceptT.bind, ExceptT.mk]; unfold ExceptT.bindCont
+    simp [MProp.ι, MPropPartialOrder.ι]
+    simp [instMPropPartialOrderExceptTOfLawfulMonad, MPropExcept, MProp.ι]
+    have h := inst'.angelic (α := Except ε α) (c := c)
+      (p := fun e =>
+        match e with
+        | Except.ok a    => p a
+        | Except.error e => ⌜True⌝ )
+      (q := fun e =>
+        match e with
+        | Except.ok a    => q a
+        | Except.error e => ⌜True⌝ )
+    simp [MProp.lift, MProp.ι, MProp.μ, MProp.μ_surjective] at h
+    have h₁ : ∀ p : α -> l,
+      (do
+        bind (m := m) c fun a =>
+        Except.getD { prop := True } <$>
+            match a with
+            | Except.ok a => Except.ok <$> MPropPartialOrder.ι (p a)
+            | Except.error e => pure (Except.error e)) =
+      (do
+        bind (m := m) c fun a =>
+        (MPropPartialOrder.ι $ match a with
+            | Except.ok a =>  (p a)
+            | Except.error e => ⌜True⌝)) := by
+      intro p; congr; ext a; cases a <;> simp
+      simp [Except.getD, MProp.pure, MProp.μ, inst.μ_pure_injective]
+    (repeat erw [h₁]); clear h₁; apply le_trans'; apply h
+    apply le_of_eq; congr; ext a; cases a <;> simp
+
+
 end PartialCorrectness
 
 namespace TotalCorrectness
@@ -109,6 +237,77 @@ scoped
 instance (ε : Type) (l : Type) (m : Type -> Type)
   [PartialOrder l]
   [Monad m] [LawfulMonad m] [inst: MPropPartialOrder m l] : MPropPartialOrder (ExceptT ε m) l := MPropExcept False ε l m
+
+def MPropExceptDetertministic (ε : Type) (l : Type) (m : Type -> Type)
+  [Lattice l]
+  [Monad m] [LawfulMonad m] [inst: MPropPartialOrder m l]
+  [inst': MPropDetertministic m l] : MPropDetertministic (ExceptT ε m) l where
+  demonic := by
+    intros α c p q
+    simp [MProp.lift, MProp.μ, MPropPartialOrder.μ]
+    simp [bind, ExceptT.bind, ExceptT.mk]; unfold ExceptT.bindCont
+    simp [MProp.ι, MPropPartialOrder.ι]
+    simp [instMPropPartialOrderExceptTOfLawfulMonad, MPropExcept, MProp.ι]
+    have h := inst'.demonic (α := Except ε α) (c := c)
+      (p := fun e =>
+        match e with
+        | Except.ok a    => p a
+        | Except.error e => ⌜False⌝ )
+      (q := fun e =>
+        match e with
+        | Except.ok a    => q a
+        | Except.error e => ⌜False⌝ )
+    simp [MProp.lift, MProp.ι, MProp.μ, MProp.μ_surjective] at h
+    have h₁ : ∀ p : α -> l,
+      (do
+        bind (m := m) c fun a =>
+        Except.getD { prop := False } <$>
+            match a with
+            | Except.ok a => Except.ok <$> MPropPartialOrder.ι (p a)
+            | Except.error e => pure (Except.error e)) =
+      (do
+        bind (m := m) c fun a =>
+        (MPropPartialOrder.ι $ match a with
+            | Except.ok a =>  (p a)
+            | Except.error e => ⌜False⌝)) := by
+      intro p; congr; ext a; cases a <;> simp
+      simp [Except.getD, MProp.pure, MProp.μ, inst.μ_pure_injective]
+    (repeat erw [h₁]); clear h₁; apply le_trans; apply h
+    apply le_of_eq; congr; ext a; cases a <;> simp
+  angelic := by
+    intros α c p q
+    simp [MProp.lift, MProp.μ, MPropPartialOrder.μ]
+    simp [bind, ExceptT.bind, ExceptT.mk]; unfold ExceptT.bindCont
+    simp [MProp.ι, MPropPartialOrder.ι]
+    simp [instMPropPartialOrderExceptTOfLawfulMonad, MPropExcept, MProp.ι]
+    have h := inst'.angelic (α := Except ε α) (c := c)
+      (p := fun e =>
+        match e with
+        | Except.ok a    => p a
+        | Except.error e => ⌜False⌝ )
+      (q := fun e =>
+        match e with
+        | Except.ok a    => q a
+        | Except.error e => ⌜ False ⌝ )
+    simp [MProp.lift, MProp.ι, MProp.μ, MProp.μ_surjective] at h
+    have h₁ : ∀ p : α -> l,
+      (do
+        bind (m := m) c fun a =>
+        Except.getD { prop := False } <$>
+            match a with
+            | Except.ok a => Except.ok <$> MPropPartialOrder.ι (p a)
+            | Except.error e => pure (Except.error e)) =
+      (do
+        bind (m := m) c fun a =>
+        (MPropPartialOrder.ι $ match a with
+            | Except.ok a =>  (p a)
+            | Except.error e => ⌜ False ⌝)) := by
+      intro p; congr; ext a; cases a <;> simp
+      simp [Except.getD, MProp.pure, MProp.μ, inst.μ_pure_injective]
+    (repeat erw [h₁]); clear h₁; apply le_trans'; apply h
+    apply le_of_eq; congr; ext a; cases a <;> simp
+
+
 end TotalCorrectness
 
 #guard_msgs (drop info) in
@@ -123,8 +322,11 @@ namespace AngelicChoice
 instance NonDetMProp :
    MPropPartialOrder NonDetM.{0} Prop where
   μ := (∃ x ∈ ·.takeAll, x.prop)
+  ι := (NonDetM.one ·)
   μ_surjective := by
-    exists (NonDetM.one ·); intros x; simp [NonDetM.takeAll]
+    intros x; simp [NonDetM.takeAll]
+  μ_pure_injective := by
+    simp [pure, NonDetM.takeAll]
   μ_top := by intros x; simp [pure, NonDetM.takeAll]
   μ_bot := by intros x; simp [pure, NonDetM.takeAll]
   μ_nontriv := by simp [pure, NonDetM.takeAll]
@@ -154,8 +356,11 @@ theorem List.forall_forall {α} (f : α -> Prop) (xs : List α) : List.forall f 
 instance NonDetMProp :
    MPropPartialOrder NonDetM.{0} Prop where
   μ := (List.forall (·.prop) ·.takeAll)
+  ι := (NonDetM.one ·)
   μ_surjective := by
-    exists (NonDetM.one ·); intros x; simp [NonDetM.takeAll]
+    intros x; simp [NonDetM.takeAll]
+  μ_pure_injective := by
+    simp [pure, NonDetM.takeAll]
   μ_top := by intros x; simp [pure, NonDetM.takeAll]
   μ_bot := by intros x; simp [pure, NonDetM.takeAll]
   μ_nontriv := by simp [pure, NonDetM.takeAll]
